theories/Validity/Properties.v
@@ -13,6 +13,7 @@ Lemma wellformedSubstEq {Γ Γ' σ σ' Δ} (VΓ : [||-v Γ ≅ Γ' ]) (wfΔ : [|
 Proof.
   revert Δ wfΔ σ σ'; indValid VΓ.
   - intros. apply conv_sempty.
+  - intros * ih ???? []. now eapply conv_sconsε, ih.
   - intros * ih ???? []. apply conv_scons.
     + now eapply ih.
     + now escape.
@@ -22,9 +23,13 @@ Lemma consSubst {Γ Γ' σ σ' t u l A A' Δ} (VΓ : [||-v Γ ≅ Γ']) (wfΔ : 
   (Vσσ' : [Δ ||-v σ ≅ σ' : Γ | VΓ | wfΔ ])
   (VA : [Γ ||-v<l> A ≅ A' | VΓ])
   (Vtu : [Δ ||-<l> t ≅ u : A[σ] | validTyExt VA wfΔ Vσσ']) :
-  [Δ ||-v (t .: σ) ≅  (u .: σ') : Γ ,, A | validSnoc VΓ VA | wfΔ ].
+  [Δ ||-v (to_subst (t..)) ∘s (up_subst σ) ≅ (to_subst (u..)) ∘s (up_subst σ') : Γ ,, A | validSnoc VΓ VA | wfΔ ].
 Proof.
   unshelve econstructor; tea.
+  + eapply irrelevanceSubstEqExt, Vσσ'; constructor;
+    cbn; unfold funcomp; cbn; now bsimpl.
+  + eapply (irrLREq (validTyExt VA wfΔ Vσσ')), Vtu.
+    eapply subst_subst_eq; constructor; cbn; unfold funcomp; cbn; now bsimpl.
 Qed.
 
 
@@ -32,11 +37,22 @@ Lemma consValidSubst {Γ Γ' σ σ' t u l A A' Δ} {VΓ : [||-v Γ ≅ Γ']} {wf
   (Vσσ' : [Δ ||-v σ ≅ σ' : Γ | VΓ | wfΔ ])
   {VA : [Γ ||-v<l> A ≅ A' | VΓ]}
   (Vt : [Γ ||-v<l> t ≅ u : A | VΓ | VA]) :
-  [Δ ||-v (t[σ] .: σ) ≅  (u[σ'] .: σ') : Γ ,, A | validSnoc VΓ VA | wfΔ ].
+  [Δ ||-v σ ∘s (to_subst t..) ≅  σ' ∘s (to_subst u..) : Γ ,, A | validSnoc VΓ VA | wfΔ ].
 Proof.
   unshelve econstructor; intros; tea.
   now apply validTmExt.
 Qed.
+
+
+(* Lemma consValidSubst {Γ Γ' σ σ' t u l A A' Δ} {VΓ : [||-v Γ ≅ Γ']} {wfΔ : [|- Δ]}
+  (Vσσ' : [Δ ||-v σ ≅ σ' : Γ | VΓ | wfΔ ])
+  {VA : [Γ ||-v<l> A ≅ A' | VΓ]}
+  (Vt : [Γ ||-v<l> t ≅ u : A | VΓ | VA]) :
+  [Δ ||-v (t[σ] .: σ) ≅  (u[σ'] .: σ') : Γ ,, A | validSnoc VΓ VA | wfΔ ].
+Proof.
+  unshelve econstructor; intros; tea.
+  now apply validTmExt.
+Qed. *)
 
 Lemma wkSubst {Γ Γ'} (VΓ : [||-v Γ ≅ Γ']) :
   forall {σ σ' Δ Δ'}  (wfΔ : [|- Δ]) (wfΔ' : [|- Δ']) (ρ : Δ' ≤ Δ),
@@ -44,13 +60,19 @@ Lemma wkSubst {Γ Γ'} (VΓ : [||-v Γ ≅ Γ']) :
   [Δ' ||-v σ ⟨ ρ ⟩ ≅ σ' ⟨ ρ ⟩ : Γ | VΓ | wfΔ' ].
 Proof.
   indValid VΓ.
-  - intros * []. constructor; eapply Fwk_compose; tea.
-    eapply ρ.
+  - intros * []. constructor.
+  - intros * ih * [htl i hhd hi hin]; unshelve econstructor.
+    + eapply ren_index, i; eapply ρ.
+    + eapply irrelevanceSubstEqExt, ih with (ρ:=ρ); tea; constructor; cbn; now bsimpl.
+    + change (subst_alpha ?σ⟨ρ⟩ 0) with (ρ.(Fwk) (subst_alpha σ 0)). now f_equal.
+    + change (subst_alpha ?σ⟨ρ⟩ 0) with (ρ.(Fwk) (subst_alpha σ 0)). rewrite ren_index_to_ren. now f_equal.
+    + intros n b hin'. eapply well_Fwk_in, hin, hin'.
   - intros * ih * [tl hd]; unshelve econstructor.
-    + eapply ih ; eassumption.
+    + eapply irrelevanceSubstEqExt, ih with (ρ:=ρ) ; tea; constructor; cbn; bsimpl; reflexivity.
     + eapply irrLREq.
       2: now unshelve now eapply wkLR.
-      now asimpl.
+      rewrite subst_ren_wk.
+      eapply subst_subst_eq. constructor; reflexivity.
 Qed.
 
 Lemma wk1Subst {Γ Γ' σ σ' Δ F} (VΓ : [||-v Γ ≅ Γ'])
@@ -62,7 +84,7 @@ Proof.
   intro vσσ'. eapply wkSubst ; eassumption.
 Qed.
 
-Lemma consWkSubst {Γ Γ' Δ Ξ A A' σ σ' a b l} {VΓ : [||-v Γ ≅ Γ']} {wfΔ : [|- Δ]}
+(* Lemma consWkSubst {Γ Γ' Δ Ξ A A' σ σ' a b l} {VΓ : [||-v Γ ≅ Γ']} {wfΔ : [|- Δ]}
   (VA : [Γ ||-v<l> A ≅ A' | VΓ])
   (Vσσ' : [Δ ||-v σ ≅ σ' : Γ | VΓ | wfΔ ])
   (ρ : Ξ ≤ Δ) wfΞ
@@ -122,8 +144,7 @@ Lemma liftSubstSym' {Γ Γ' σ σ' Δ lF F F'} {VΓ : [||-v Γ ≅ Γ' ]} {wfΔ 
 Proof.
   unshelve eapply irrelevanceSubst, liftSubst'; cycle 3; [now eapply symValidTy'|..]; tea.
   now eapply symSubst.
-Qed.
-
+Qed. *)
 
 
 
@@ -131,8 +152,8 @@ Lemma wk1ValidTy {Γ Γ' lA A A' lF F F'} {VΓ : [||-v Γ ≅ Γ']} (VF : [Γ ||
   [Γ ||-v<lA> A ≅ A' | VΓ] ->
   [Γ ,, F ||-v<lA> A ⟨ @wk1 Γ F ⟩ ≅ A' ⟨ @wk1 Γ' F' ⟩ | validSnoc VΓ VF ].
 Proof.
-  intros VA; constructor; intros * [tl hd].
-  rewrite 2!wk1_subst; now eapply validTyExt.
+  intros VA; constructor; intros * [hd tl].
+  rewrite 2wk1_subst; now eapply validTyExt.
 Qed.
 
 Lemma wk1ValidTm {Γ Γ' lA t u A A' lF F F'} {VΓ : [||-v Γ ≅ Γ']}
@@ -165,37 +186,52 @@ Proof.
 Defined.
 
 Lemma soundCtxId {Γ Γ'} (VΓ : [||-v Γ ≅ Γ']) :
-  ∑ wfΓ : [|- Γ], [Γ ||-v tRel : Γ | VΓ | wfΓ].
+  ∑ wfΓ : [|- Γ], [Γ ||-v subst_id : Γ | VΓ | wfΓ].
 Proof.
   indValid VΓ.
   - intros; eexists wfc_nil; constructor.
-    eapply Fwk_id.
+  - intros ?????? VΓ VF [wfΓ ih].
+    pose (wfΓF := wfc_consε (F:=F) wfΓ).
+(*     pose proof (RA := validTyExt VA _ ih). *)
+(*     assert (hA : [Γ |- A]) by (rewrite <- subst_rel; exact (escapeSplit RA)). *)
+(*     pose (wfΓA := wfc_cons wfΓ hA). *)
+    exists wfΓF.
+    unshelve econstructor.
+    + eapply index_0.
+    + eapply irrelevanceSubstEqExt,
+        wkSubst with (ρ:=wk_alphastep F (@wk_id Γ)), ih;
+        constructor; cbn; bsimpl; reflexivity.
+    + reflexivity.
+    + reflexivity.
+    + eapply Fwk_id.
   - intros ????? VΓ VA [wfΓ ih].
     pose proof (RA := validTyExt VA _ ih).
-    assert (hA : [Γ |- A]) by (rewrite <- subst_rel; exact (escapeSplit RA)).
+    assert (hA : [Γ |- A]) by (rewrite subst_id_on; exact (escapeSplit RA)).
     pose (wfΓA := wfc_cons wfΓ hA).
-    assert (Vs : [VΓ | _ ||-v ↑ >> tRel : _ | wfΓA]).
+    assert (Vs : [VΓ | _ ||-v tail_subst subst_id : _ | wfΓA]).
     1:{
-      eapply irrelevanceSubstEqExt.
-      3: eapply (wkSubst _ _ _ (@wk1 Γ A)), ih.
-      all: intros ?; now bsimpl.
+      eapply irrelevanceSubstEqExt, wkSubst with (ρ := @wk1 Γ A), ih;
+        constructor; cbn; bsimpl; try reflexivity; tea.
     }
     exists wfΓA; exists Vs.
     eapply var0; tea.
-    rewrite <-(subst_rel A⟨↑⟩); now asimpl.
+    now rewrite <- wk1_subst with (A:= A) (Γ:=Γ), <- subst_id_on.
 Qed.
 
 
 Definition escapeValid {Γ Γ'} (VΓ : [||-v Γ ≅ Γ']) : [|-Γ] := (soundCtxId VΓ).π1.
 
-Definition idSubst {Γ Γ'} (VΓ : [||-v Γ ≅ Γ']) : [Γ ||-v tRel : Γ | VΓ | _] := (soundCtxId VΓ).π2.
+Definition idSubst {Γ Γ'} (VΓ : [||-v Γ ≅ Γ']) : [Γ ||-v subst_id : Γ | VΓ | _] := (soundCtxId VΓ).π2.
 
 Lemma redValidTy {Γ Γ' A A' l} {VΓ : [||-v Γ ≅ Γ']} (vA : [_ ||-v<l> A ≅ A' | VΓ ]) : [Γ ||-<l> A ≅ A'].
-Proof. intros; instValid (idSubst VΓ); now rewrite !subst_rel in *. Qed.
+Proof. intros; instValid (idSubst VΓ); now rewrite <- !subst_id_on in *. Qed.
 
 Lemma redValidTm {Γ Γ' A A' l t t'} {VΓ : [||-v Γ ≅ Γ']} {VA : [_ ||-v<l> A ≅ A' | VΓ ]}
   (Vt : [Γ ||-v<l> t ≅ t' : _ | _ | VA]) :  [Γ ||-<l> t ≅ t' : _ | redValidTy VA ].
-Proof. intros; instValid (idSubst VΓ); rewrite !subst_rel, !(subst_rel t) in *; eapply irrLREq; tea; now apply subst_rel. Qed.
+Proof.
+  intros; instValid (idSubst VΓ); rewrite <- !subst_id_on, <- !(subst_id_on t) in *; eapply irrLREq; tea;
+  now rewrite subst_id_on.
+Qed.
 
 Lemma redValidTm' {Γ Γ' A A' l t t'} {VΓ : [||-v Γ ≅ Γ']} {VA : [_ ||-v<l> A ≅ A' | VΓ ]}
   (RA : [Γ ||-<l> A ≅ A']) (Vt : [Γ ||-v<l> t ≅ t' : _ | _ | VA]) :  [Γ ||-<l> t ≅ t' : _ | RA].
@@ -204,31 +240,29 @@ Proof. now eapply irrLR, redValidTm. Qed.
 
 Lemma wkrenSubst {Γ Δ} (ρ : Δ ≤ Γ) :
   forall {Γ' Δ'} (VΓ : [||-v Γ ≅ Γ']) (VΔ : [||-v Δ ≅ Δ'])  {Ξ σ σ'} (wfΞ : [|- Ξ]),
-  [VΔ | Ξ ||-v σ ≅ σ' : _ | wfΞ] -> [VΓ | Ξ ||-v ρ >> σ ≅ ρ >> σ' : _ | wfΞ].
+  [VΔ | Ξ ||-v σ ≅ σ' : _ | wfΞ] -> [VΓ | Ξ ||-v ρ >>s σ ≅ ρ >>s σ' : _ | wfΞ].
 Proof.
-  destruct Γ as [Γ L], Δ as [Δ LΔ].
-  destruct ρ as [? wwk ?]; cbn in *; induction wwk.
-  + intros *.
-    pose proof (invValidity VΓ) as (?&?&e&h); subst; cbn in h; subst.
-    pose proof (invValidity VΔ) as (?&?&e&h); subst; cbn in h; subst.
-    intros []; constructor.
-    now eapply Fwk_compose.
-  + intros * Vσ.
-    pose proof (invValidity VΔ) as (?&?&?&?&?&e&h); subst; cbn in h; subst.
-    destruct Vσ as [tl hd].
-    eapply irrelevanceSubstEqExt.
-    3: eapply IHwwk, tl.
-    - rewrite <- (scons_eta' σ) at 1; reflexivity.
-    - rewrite <- (scons_eta' σ') at 1; reflexivity.
-  + intros * Vσ.
-    pose proof (invValidity VΔ) as (?&?&?&?&?&e&h); subst; cbn in h; subst.
+  induction ρ using wk_induction; intros * Vσ.
+  + pose proof (invValidity VΓ) as (e&h); subst; cbn in h; subst.
+    constructor.
+  + pose proof (invValidity VΔ) as (?&?&?&?&?&e&h); subst; cbn in h; subst.
+    destruct Vσ as [htl hhd].
+    eapply (IHρ _ _ _ _ _ _ _ _ htl).
+  + pose proof (invValidity VΔ) as (?&?&?&?&?&e&h); subst; cbn in h; subst.
     pose proof (invValidity VΓ) as (?&?&?&?&?&e&h); subst; cbn in h; subst.
-    destruct Vσ as [tl hd].
-    eapply irrelevanceSubstEqExt.
-    1:{ rewrite <- (scons_eta' σ); cbn; unfold up_ren; rewrite scons_comp'; cbn. reflexivity. }
-    1:{ rewrite <- (scons_eta' σ'); cbn; unfold up_ren; rewrite scons_comp'; cbn. reflexivity. }
-    opector; [now eapply IHwwk|].
-    cbn;  eapply irrLREqCum; tea; now bsimpl.
+    destruct Vσ as [tl hd]. opector.
+    - refine (IHρ _ _ _ _ _ _ _ _ tl).
+    - eapply irrLREqCum; tea;
+      now rewrite wk_subst_comp_on.
+  + pose proof (invValidity VΔ) as (?&?&?&?&e&h); subst; cbn in h; subst.
+    destruct Vσ as [htl i hd hi hin].
+    eapply (IHρ _ _ _ _ _ _ _ _ htl).
+  + pose proof (invValidity VΔ) as (?&?&?&?&e&h); subst; cbn in h; subst.
+    pose proof (invValidity VΓ) as (?&?&?&?&e&h); subst; cbn in h; subst.
+    destruct Vσ as [htl i hd hi hin].
+    econstructor; tea.
+    - refine (IHρ _ _ _ _ _ _ _ _ htl).
+    - now eapply Fwk_compose.
 Qed.
 
 Lemma wkValidTy {l Γ Γ' Δ Δ' A A'} (ρ : Δ ≤ Γ)
@@ -237,7 +271,7 @@ Lemma wkValidTy {l Γ Γ' Δ Δ' A A'} (ρ : Δ ≤ Γ)
   (VA : [Γ ||-v<l> A ≅ A' | VΓ]) :
   [Δ ||-v<l> A⟨ρ⟩ ≅ A'⟨ρ⟩ | VΔ].
 Proof.
-  constructor; intros; cbn; rewrite !ren_subst.
+  constructor; intros; cbn; rewrite !wk_subst_comp_on.
   eapply validTyExt; tea; now eapply wkrenSubst.
 Qed.
 
@@ -248,14 +282,14 @@ Lemma wkValidTm {l Γ Γ' Δ Δ' A A' t u} (ρ : Δ ≤ Γ)
   (Vt : [Γ ||-v<l> t ≅ u: A | VΓ | VA]) :
   [Δ ||-v<l> t⟨ρ⟩ ≅ u⟨ρ⟩ : A⟨ρ⟩ | VΔ | wkValidTy ρ VΓ VΔ VA].
 Proof.
-  econstructor; intros; rewrite !ren_subst, !(ren_subst t).
-  (unshelve now eapply irrLREq, validTmExt; tea; rewrite ren_subst); tea.
+  econstructor; intros; rewrite !wk_subst_comp_on, !wk_subst_comp_on with (t:=t).
+  (unshelve now eapply irrLREq, validTmExt; tea; rewrite wk_subst_comp_on); tea.
   now eapply wkrenSubst.
 Qed.
 
 Lemma escapeValidTy {Γ Γ' A A' l} (VΓ : [||-v Γ ≅ Γ']) : [_ ||-v<l> A ≅ A' | VΓ ] -> [Γ |- A] × [Γ |- A'] × [Γ |-  A ≅ A'].
 Proof.
-  intros VA;  generalize (validTyExt VA _ (idSubst VΓ)); rewrite 2!subst_rel; intros; now escape.
+  intros VA;  generalize (validTyExt VA _ (idSubst VΓ)); rewrite <- 2!subst_id_on; intros; now escape.
 Qed.
 
 Lemma escapeValidTm {Γ Γ' A A' l t t'} (VΓ : [||-v Γ ≅ Γ'])
@@ -263,7 +297,7 @@ Lemma escapeValidTm {Γ Γ' A A' l t t'} (VΓ : [||-v Γ ≅ Γ'])
   [_ ||-v<l> t ≅ t' : _ | _ | VA] -> [Γ |- t : A] × [Γ |- t' : A] × [Γ |- t ≅ t' : A].
 Proof.
   intros Vt; pose proof (validTmExt Vt _ (idSubst VΓ)); escape.
-  rewrite !subst_rel in *. now repeat split.
+  rewrite <- !subst_id_on in *. now repeat split.
 Qed.
 
 Lemma redSubstValid {Γ Γ' A A' t u l}
@@ -284,7 +318,7 @@ Lemma SsubstS {Γ Γ' F F' G G' t t' l} {VΓ : [||-v Γ ≅ Γ']}
   (Vt : [Γ ||-v<l> t ≅ t' : F | VΓ | VF]) :
   [Γ ||-v<l> G[t..] ≅ G'[t'..] | VΓ].
 Proof.
-  constructor; intros; rewrite 2!singleSubstComm.
+  constructor; intros. rewrite 2to_subst_sound, 2subst_comp_on.
   eapply validTyExt; tea; now eapply consValidSubst.
 Qed.
 
@@ -294,8 +328,8 @@ Lemma substS {Γ Γ' F F' G G' t t' l} {VΓ : [||-v Γ ≅ Γ']}
   (Vt : [Γ ||-v<l> t ≅ t' : F | VΓ | VF]) :
   [Γ ||-v<l> G[t..] ≅ G'[t'..] | VΓ].
 Proof.
-  constructor; intros; rewrite 2!singleSubstComm.
-  eapply validTyExt; tea. now eapply consValidSubst.
+  constructor; intros. rewrite 2to_subst_sound, 2subst_comp_on.
+  eapply validTyExt; tea; now eapply consValidSubst.
 Qed.
 
 Lemma substSTm {Γ Γ' F F' G G' t t' f f' l} (VΓ : [||-v Γ ≅ Γ'])
@@ -306,9 +340,12 @@ Lemma substSTm {Γ Γ' F F' G G' t t' f f' l} (VΓ : [||-v Γ ≅ Γ'])
   (Vff' : [Γ ,, F ||-v<l> f ≅ f' : G | VΓF | VG]) :
   [Γ ||-v<l> f[t..] ≅ f'[t'..] : G[t..] | VΓ | substS VG Vtt'].
 Proof.
-  constructor; intros; rewrite !singleSubstComm, !(singleSubstComm f).
+  constructor; intros.
+  replace f[t..][σ] with f[σ ∘s to_subst t..].
+  replace f'[t'..][σ'] with f'[σ' ∘s to_subst t'..].
+  2,3: now rewrite to_subst_sound, subst_comp_on.
   eapply irrLREq.
-  1: symmetry; apply singleSubstComm.
+  1: symmetry; now rewrite to_subst_sound, subst_comp_on.
   (unshelve now eapply validTmExt); tea.
   now eapply consValidSubst.
 Qed.
@@ -335,12 +372,13 @@ Lemma substLiftS {Γ Γ' F F' G G' A A' t t' l} (VΓ : [||-v Γ ≅ Γ'])
   (VG : [Γ,, A ||-v<l> G ≅ G' | VΓA])
   (VA' := wk1ValidTy VF VA)
   (Vt : [Γ,, F ||-v<l> t ≅ t' : A⟨@wk1 Γ F⟩ | VΓF | VA']) :
-  [Γ ,, F ||-v<l> G[t]⇑ ≅ G'[t']⇑ | VΓF].
+  [Γ ,, F ||-v<l> G⟨wk_up A (@wk1 Γ F)⟩[t..] ≅ G'⟨wk_up A' (@wk1 Γ F)⟩[t'..] | VΓF].
 Proof.
-  constructor; intros; erewrite 2! liftSubstComm.
-  eapply validTyExt; tea; opector.
+  constructor; intros.
+  rewrite 2!to_subst_sound, 2subst_comp_on, 2wk_subst_comp_on.
+  eapply validTyExt; tea. opector.
   1: now eapply wkrenSubst.
-  now unshelve now eapply irrLREq, validTmExt; tea; rewrite ren_subst.
+  now unshelve now eapply irrLREq, validTmExt; tea; rewrite wk_subst_comp_on.
 Qed.
 
 
